theories/ordinals/Ackermann/ListExt.v
@@ -1,5 +1,5 @@
 (**  Replaced some proofs with Stdlib's 
-     Provisionally, we still export original names 
+     Provisionally, we still export original lemma names 
  *)
 
 Require Import Coq.Lists.List.
@@ -9,54 +9,26 @@ Section List_Remove.
 Variable A : Set.
 Hypothesis Aeq_dec : forall a b : A, {a = b} + {a <> b}.
 
-Fixpoint list_remove (x : A) (l : list A) : list A :=
-  match l with
-    nil => l
-  | a::l => match Aeq_dec a x with
-            | left _ => list_remove x l
-            | right _ => a :: list_remove x l
-            end
-  end.
 
-Print List.remove. 
-
-Lemma list_remove_compat x l  :
-  list_remove x l = List.remove Aeq_dec x l.
-Proof.
-  induction l.
-  - reflexivity. 
-  -  simpl; case (Aeq_dec a x) ; simpl; intros; subst. 
-     + case (Aeq_dec x x) ; now rewrite IHl. 
-     + case (Aeq_dec x a).
-       * subst; congruence. 
-       * now rewrite IHl. 
-Qed. 
-
-
+(* to deprecate *)
 Lemma In_list_remove1 :
- forall (a b : A) (l : list A), In a (list_remove b l) -> In a l.
+ forall (a b : A) (l : list A), In a (List.remove Aeq_dec b l) -> In a l.
 Proof.
-  intros a b l H; rewrite list_remove_compat in H.
-  now destruct (in_remove _ _ _ _ H).
+  intros a b l H; now destruct (in_remove _ _ _ _ H).
 Qed.
 
 Lemma In_list_remove2 :
- forall (a b : A) (l : list A), In a (list_remove b l) -> a <> b.
+ forall (a b : A) (l : list A), In a (List.remove Aeq_dec b l) -> a <> b.
 Proof.
-  intros a b l H; rewrite list_remove_compat in H.
-  now destruct (in_remove _ _ _ _ H).
+  intros a b l H; now destruct (in_remove _ _ _ _ H).
 Qed.
-
-
-
 
 Lemma In_list_remove3 :
   forall (a b : A) (l : list A), 
-    In a l -> a <> b -> In a (list_remove b l).
+    In a l -> a <> b -> In a (List.remove Aeq_dec b l).
   Proof. 
-    intros; rewrite list_remove_compat; now apply in_in_remove. 
+    intros; now apply in_in_remove. 
 Qed. 
 
 End List_Remove.
-
 
